\documentclass[12pt]{article}
\usepackage{amsmath}
\usepackage{graphicx}
\usepackage{hyperref}
\usepackage[utf8]{inputenc}

\title{Chapter 1: Untyped Lambda Calculus}
\author{Type Theory and Formal Proof Reading Group}
\date{}

\begin{document}

\maketitle
1.1 Apply Notation 1.3.10 on the following $\lambda$-terms. So, remove parentheses and combine $\lambda$-abstractions:

(a) $(\lambda x . (((x z) y) (x x)))$

(b) $((\lambda x . (\lambda y . (\lambda z . (z ((x y) z))))) (\lambda u . u))$

\vspace{1em}


\textbf{Solutions:}

\textbf{(a)}
Original term:
\[
(\lambda x . (((x z) y) (x x)))
\]

Applying Notation 1.3.10:
\[
(\lambda x . (((x z) y) (x x))) \implies \lambda x . (((x z) y) (x x)) \implies \lambda x . (((x z) y) (x x))
\]

\textbf{(b)}
Original term:
\[
((\lambda x . (\lambda y . (\lambda z . (z ((x y) z))))) (\lambda u . u))
\]

Applying Notation 1.3.10:
% First, we substitute \( \lambda u . u \) for \( x \):
\[
((\lambda x . (\lambda y . (\lambda z . (z ((x y) z))))) (\lambda u . u)) \implies
(\lambda x . (\lambda y . (\lambda z . (z ((x y) z))))) (\lambda u . u)
\]

Now simplify:\\
\begin{align*}
   (\lambda x . (\lambda y . (\lambda z . (z ((x y) z))))) (\lambda u . u) [x = \lambda u . u] \\
   &= (\lambda y . (\lambda z . (z (((\lambda u . u) y) z)))) \\
   &= (\lambda y . (\lambda z . (z (((\lambda u . u) y) z)))) [u = y] \\
   &= \lambda y . (\lambda z . (z (y z)))
\end{align*}


\end{document}
